Unfold: work on semantics lemmas

Pdl/Unfold.lean
@@ -6,6 +6,7 @@ import Pdl.Discon
 
 -- TODO: move to Syntax.lean
 mutual
+  /-- Replace atomic proposition `x` by `ψ` in a formula. -/
   @[simp]
   def repl_in_F (x : Char) (ψ : Formula) : Formula → Formula
     | ⊥ => ⊥
@@ -13,6 +14,7 @@ mutual
     | ~φ => ~(repl_in_F x ψ φ)
     | φ1⋀φ2 => (repl_in_F x ψ) φ1 ⋀ (repl_in_F x ψ) φ2
     | ⌈α⌉ φ => ⌈repl_in_P x ψ α⌉ (repl_in_F x ψ φ)
+  /-- Replace atomic proposition `x` by `ψ` in a program. -/
   @[simp]
   def repl_in_P (x : Char) (ψ : Formula) : Program → Program
     | ·c => ·c
@@ -61,14 +63,66 @@ end
 
 -- TODO: move to Semantics?
 
-mutual
-theorem repl_in_F_equiv x ψ :
-    (φ1 ≡ φ2) → (repl_in_F x ψ φ1) ≡ (repl_in_F x ψ φ2) := sorry -- TODO easy?
+/-- Overwrite the valuation of `x` with the current value of `ψ` in a model. -/
+def repl_in_model (x : Char) (ψ : Formula) : KripkeModel W → KripkeModel W
+| M@⟨V,R⟩ => ⟨fun w c => if c == x then (M,w) ⊨ ψ else V w c,R⟩
 
-theorem repl_in_P_equiv x ψ :
-    (α1 ≡ᵣ α2) → (repl_in_P x ψ α1) ≡ᵣ (repl_in_P x ψ α2) := sorry -- TODO easy?
+mutual
+theorem repl_in_model_sat_iff x ψ φ {W} (M : KripkeModel W) (w : W) :
+    (M, w) ⊨ repl_in_F x ψ φ ↔ (repl_in_model x ψ M, w) ⊨ φ := by
+  cases φ
+  case bottom =>
+    simp [evaluatePoint, modelCanSemImplyForm]
+  case atom_prop c =>
+    simp [evaluatePoint, modelCanSemImplyForm, evaluate, repl_in_model]
+    sorry
+  case neg φ =>
+    have IH := repl_in_model_sat_iff x ψ φ M w
+    simp [evaluatePoint, modelCanSemImplyForm] at *
+    tauto
+  case and φ1 φ2 =>
+    have IH1 := repl_in_model_sat_iff x ψ φ1 M w
+    have IH2 := repl_in_model_sat_iff x ψ φ2 M w
+    simp [evaluatePoint, modelCanSemImplyForm] at *
+    rw [IH1, IH2]
+  case box α φ =>
+    have IHα := repl_in_model_rel_iff x ψ α M w
+    simp [evaluatePoint, modelCanSemImplyForm] at *
+    constructor
+    all_goals
+      intro hyp v rel
+      have IHφ := repl_in_model_sat_iff x ψ φ M v
+      specialize IHα v
+      specialize hyp v
+      tauto
+
+theorem repl_in_model_rel_iff x ψ α {W} (M : KripkeModel W) (w v : W) :
+    relate M (repl_in_P x ψ α) w v ↔ relate (repl_in_model x ψ M) α w v := by
+  sorry
 end
 
+theorem repl_in_F_equiv x ψ :
+    (φ1 ≡ φ2) → (repl_in_F x ψ φ1) ≡ (repl_in_F x ψ φ2) := by
+  intro hyp
+  intro W M w
+  have claim1 := repl_in_model_sat_iff x ψ φ1 M w
+  have claim2 := repl_in_model_sat_iff x ψ φ2 M w
+  simp only [evaluatePoint, modelCanSemImplyForm] at *
+  rw [claim1]
+  rw [claim2]
+  have := @equiv_iff φ1 φ2 hyp W (repl_in_model x ψ M) w
+  simp only [evaluatePoint, modelCanSemImplyForm] at *
+  exact this
+
+theorem repl_in_P_equiv x ψ :
+    (α1 ≡ᵣ α2) → (repl_in_P x ψ α1) ≡ᵣ (repl_in_P x ψ α2) := by
+  intro hyp
+  intro W M w v
+  have claim1 := repl_in_model_rel_iff x ψ α1 M w v
+  have claim2 := repl_in_model_rel_iff x ψ α2 M w v
+  rw [claim1]
+  rw [claim2]
+  apply hyp
 
 -- ### Test Profiles
 
